WIP

mem/MemOpenWhole.v
@@ -27,12 +27,18 @@ Notation "(∘)" := (fun g f => g ∘ f) (at level 40, left associativity).
 Section AUX.
   Context `{Σ: GRA.t}.
   Definition fspec_trivial: fspec := (mk_simple (fun (_: unit) => (fun _ _ => ⌜True⌝, fun _ => ⌜True⌝))).
+
 End AUX.
 
 
 
-Module CModSem.
-Section CMODSEM.
+
+(******************************************* UNKNOWN ***********************************************)
+(******************************************* UNKNOWN ***********************************************)
+(******************************************* UNKNOWN ***********************************************)
+
+Module UModSem.
+Section UMODSEM.
 
   Context `{Σ: GRA.t}.
 
@@ -81,44 +87,202 @@ Section CMODSEM.
   |}
   .
 
-End CMODSEM.
-End CModSem.
+End UMODSEM.
+End UModSem.
 
 
 
 
-Module CMod.
-Section CMOD.
+Module UMod.
+Section UMOD.
 
   Context `{Σ: GRA.t}.
 
   Record t: Type := mk {
-    get_modsem: SkEnv.t -> CModSem.t;
+    get_modsem: SkEnv.t -> UModSem.t;
     sk: Sk.t;
   }
   .
 
   Definition to_mod (md: t): Mod.t := {|
-    Mod.get_modsem := CModSem.to_modsem ∘ md.(get_modsem);
+    Mod.get_modsem := UModSem.to_modsem ∘ md.(get_modsem);
     Mod.sk := md.(sk);
   |}
   .
 
-  Lemma to_mod_comm: forall md skenv, CModSem.to_modsem (md.(get_modsem) skenv) = (to_mod md).(Mod.get_modsem) skenv.
+  Lemma to_mod_comm: forall md skenv, UModSem.to_modsem (md.(get_modsem) skenv) = (to_mod md).(Mod.get_modsem) skenv.
   Proof. i. refl. Qed.
 
 
   Definition to_smod (md: t): SMod.t := {|
-    SMod.get_modsem := CModSem.to_smodsem ∘ md.(get_modsem);
+    SMod.get_modsem := UModSem.to_smodsem ∘ md.(get_modsem);
     SMod.sk := md.(sk);
   |}
   .
 
-  Lemma to_smod_comm: forall md skenv, CModSem.to_smodsem (md.(get_modsem) skenv) = (to_smod md).(SMod.get_modsem) skenv.
+  Lemma to_smod_comm: forall md skenv, UModSem.to_smodsem (md.(get_modsem) skenv) = (to_smod md).(SMod.get_modsem) skenv.
   Proof. i. refl. Qed.
 
-End CMOD.
-End CMod.
+End UMOD.
+End UMod.
+
+
+
+
+
+
+
+
+
+
+
+
+
+
+
+
+
+
+
+
+
+(********************************************* KNOWN ***********************************************)
+(********************************************* KNOWN ***********************************************)
+(********************************************* KNOWN ***********************************************)
+
+Section AUX.
+  Context `{Σ: GRA.t}.
+
+  Record fspecbodyk: Type := mk_fsbk {
+    fsbk_fspec:> fspec;
+    (* fsbk_body: (fsbk_fspec.(AA) * bool) -> itree (hCallE +' pE +' eventE) fsbk_fspec.(AR); *)
+    (*** <--- this is not handy when removing the "is_k" argument at the top level ***)
+
+    (* fsbk_bodyk: fsbk_fspec.(AA) -> itree (hCallE +' pE +' eventE) fsbk_fspec.(AR); *)
+    (* fsbk_bodyu: fsbk_fspec.(AA) -> itree (hCallE +' pE +' eventE) fsbk_fspec.(AR); *)
+    (*** <--- do we need fsbk_bodyk at all? it will always be APC (or just choose) because the k-cases will all be removed ***)
+
+    fsbk_bodyu: fsbk_fspec.(AA) -> itree (hCallE +' pE +' eventE) fsbk_fspec.(AR);
+    (*** <--- Now fspecbodyk has the same type with fspecbody! we don't need this definition ***)
+  }
+  .
+
+  Definition disclose (fs: fspec): fspec :=
+    @mk _ (fs.(X) * bool)%type (fs.(AA) * bool)%type (fs.(AR))
+        (fun '(x, is_k) '(argh, is_k') argl o => ⌜is_k = is_k'⌝ ** (⌜is_k⌝ -* fs.(precond) x argh argl o ** ⌜is_pure o⌝))
+        (fun '(x, is_k) reth retl =>                               (⌜is_k⌝ -* fs.(postcond) x reth retl))
+  .
+
+  Definition disclose_fsbk (fsbk: fspecbodyk): fspecbody :=
+    mk_specbody (disclose fsbk) fsbk.(fsbk_body)
+  .
+
+  Definition disclose_smodsem (ms: SModSem.t): SModSem.t := {|
+    SModSem.fnsems
+  |}
+  .
+
+  Definition expose_smod (md: SMod.t): SMod.t.
+
+End AUX.
+
+Module KModSem.
+Section KMODSEM.
+
+  Context `{Σ: GRA.t}.
+
+  Record t: Type := mk {
+    fnsems: list (gname * (list val -> itree (callE +' pE +' eventE) val));
+    mn: mname;
+    initial_st: Any.t;
+  }
+  .
+
+  Definition to_modsem (ms: t): ModSem.t := {|
+    (* ModSem.fnsems := List.map (map_snd (fun ktr arg => resum_itr (T:=Any.t) (cfun ktr arg))) ms.(fnsems); *)
+    (* ModSem.fnsems := List.map (map_snd (fun ktr => resum_itr (T:=Any.t) ∘ cfun ktr)) ms.(fnsems); *)
+    ModSem.fnsems := List.map (map_snd (((∘)∘(∘)) (resum_itr (T:=Any.t)) cfun)) ms.(fnsems);
+    ModSem.mn := ms.(mn);
+    ModSem.initial_mr := ε;
+    ModSem.initial_st := ms.(initial_st);
+  |}
+  .
+
+
+
+
+  Definition transl_callE: callE ~> hCallE :=
+    fun T '(Call fn args) => hCall false fn args
+  .
+
+  Definition transl_event: (callE +' pE +' eventE) ~> (hCallE +' pE +' eventE) :=
+    (bimap transl_callE (bimap (id_ _) (id_ _)))
+  .
+
+  Definition transl_itr: (callE +' pE +' eventE) ~> itree (hCallE +' pE +' eventE) :=
+    embed ∘ transl_event
+  .
+
+  Definition transl_fun: (list val -> itree (callE +' pE +' eventE) val) -> fspecbody :=
+    fun ktr =>
+      mk_specbody fspec_trivial (interp (T:=val) transl_itr ∘ ktr)
+  .
+
+  Definition to_smodsem (ms: t): SModSem.t := {|
+    SModSem.fnsems := List.map (map_snd transl_fun) ms.(fnsems);
+    SModSem.mn := ms.(mn);
+    SModSem.initial_mr := ε;
+    SModSem.initial_st := ms.(initial_st);
+  |}
+  .
+
+End KMODSEM.
+End KModSem.
+
+
+
+
+Module KMod.
+Section KMOD.
+
+  Context `{Σ: GRA.t}.
+
+  Record t: Type := mk {
+    get_modsem: SkEnv.t -> UModSem.t;
+    sk: Sk.t;
+  }
+  .
+
+  Definition to_mod (md: t): Mod.t := {|
+    Mod.get_modsem := UModSem.to_modsem ∘ md.(get_modsem);
+    Mod.sk := md.(sk);
+  |}
+  .
+
+  Lemma to_mod_comm: forall md skenv, UModSem.to_modsem (md.(get_modsem) skenv) = (to_mod md).(Mod.get_modsem) skenv.
+  Proof. i. refl. Qed.
+
+
+  Definition to_smod (md: t): SMod.t := {|
+    SMod.get_modsem := UModSem.to_smodsem ∘ md.(get_modsem);
+    SMod.sk := md.(sk);
+  |}
+  .
+
+  Lemma to_smod_comm: forall md skenv, UModSem.to_smodsem (md.(get_modsem) skenv) = (to_smod md).(SMod.get_modsem) skenv.
+  Proof. i. refl. Qed.
+
+End KMOD.
+End KMod.
+
+
+
+
+
+
+
+
+
 
 
 
@@ -132,23 +296,23 @@ Section ADQ.
   Context `{Σ: GRA.t}.
 
   Variable mds: list SMod.t.
-  Variable ctxs: list CMod.t.
+  Variable ctxs: list UMod.t.
 
-  Let sk_link: Sk.t := fold_right Sk.add Sk.unit ((List.map SMod.sk mds) ++ (List.map CMod.sk ctxs)).
+  Let sk_link: Sk.t := fold_right Sk.add Sk.unit ((List.map SMod.sk mds) ++ (List.map UMod.sk ctxs)).
   Let skenv: SkEnv.t := Sk.load_skenv sk_link.
 
   Let imss: list SModSem.t := List.map (flip SMod.get_modsem skenv) mds.
-  Let emss: list CModSem.t := List.map (flip CMod.get_modsem skenv) ctxs.
+  Let emss: list UModSem.t := List.map (flip UMod.get_modsem skenv) ctxs.
 
   Let gstb: list (gname * fspec) :=
     (flat_map (List.map (map_snd fsb_fspec) ∘ SModSem.fnsems) imss)
-      ++ (flat_map (List.map (map_snd (fun _ => fspec_trivial)) ∘ CModSem.fnsems) emss).
+      ++ (flat_map (List.map (map_snd (fun _ => fspec_trivial)) ∘ UModSem.fnsems) emss).
 
   Lemma my_lemma1
         ctx
         (IN: In ctx ctxs)
     :
-      ModPair.sim (SMod.to_tgt gstb (CMod.to_smod ctx)) (CMod.to_mod ctx)
+      ModPair.sim (SMod.to_tgt gstb (UMod.to_smod ctx)) (UMod.to_mod ctx)
   .
   Proof.
     admit "somehow".
@@ -158,12 +322,12 @@ Section ADQ.
   (*       ctx *)
   (*       (IN: In ctx ctxs) *)
   (*   : *)
-  (*     ModPair.sim (CMod.to_mod ctx) (SMod.to_tgt gstb (CMod.to_smod ctx)) *)
+  (*     ModPair.sim (UMod.to_mod ctx) (SMod.to_tgt gstb (UMod.to_smod ctx)) *)
   (* . *)
   (* Proof. *)
   (* Qed. *)
 
-  Lemma sk_link_eq: sk_link = (fold_right Sk.add Sk.unit (List.map SMod.sk (mds ++ List.map CMod.to_smod ctxs))).
+  Lemma sk_link_eq: sk_link = (fold_right Sk.add Sk.unit (List.map SMod.sk (mds ++ List.map UMod.to_smod ctxs))).
   Proof.
     unfold sk_link. f_equal. rewrite List.map_app. f_equal. rewrite List.map_map. ss.
   Qed.
@@ -179,8 +343,8 @@ Section ADQ.
     (List.map (fun '(fn, fs) => (fn, fs.(fsb_fspec)))
        (flat_map SModSem.fnsems
           (List.map
-             (flip SMod.get_modsem (Sk.load_skenv (fold_right Sk.add Sk.unit (List.map SMod.sk (mds ++ List.map CMod.to_smod ctxs)))))
-             (mds ++ List.map CMod.to_smod ctxs))))
+             (flip SMod.get_modsem (Sk.load_skenv (fold_right Sk.add Sk.unit (List.map SMod.sk (mds ++ List.map UMod.to_smod ctxs)))))
+             (mds ++ List.map UMod.to_smod ctxs))))
   .
   Proof.
     rewrite <- sk_link_eq. folder. unfold gstb.
@@ -209,8 +373,8 @@ Section ADQ.
   Hypothesis MAINM: In (SMod.main mainpre mainbody) mds.
 
   Theorem adequacy_open:
-    refines_closed (Mod.add_list (List.map (SMod.to_tgt gstb) mds ++ List.map CMod.to_mod ctxs))
-                   (Mod.add_list (List.map SMod.to_src mds ++ List.map CMod.to_mod ctxs))
+    refines_closed (Mod.add_list (List.map (SMod.to_tgt gstb) mds ++ List.map UMod.to_mod ctxs))
+                   (Mod.add_list (List.map SMod.to_src mds ++ List.map UMod.to_mod ctxs))
   .
   Proof.
     etrans.
@@ -218,18 +382,18 @@ Section ADQ.
       rewrite Mod.add_list_app.
       eapply refines_proper_l.
       eapply adequacy_local_list.
-      instantiate (1:=(List.map (SMod.to_tgt gstb ∘ CMod.to_smod) ctxs)).
+      instantiate (1:=(List.map (SMod.to_tgt gstb ∘ UMod.to_smod) ctxs)).
       eapply Forall2_apply_Forall2.
       { instantiate (1:=eq). admit "ez - generalize this lemma to iff: Forall2_eq". }
       i. subst. eapply my_lemma1; ss.
     }
     rewrite <- Mod.add_list_app.
     etrans.
-    { rewrite <- List.map_map with (f:=CMod.to_smod).
+    { rewrite <- List.map_map with (f:=UMod.to_smod).
       rewrite <- map_app.
       eapply adequacy_type2.
-      - instantiate (1:=(mds ++ List.map CMod.to_smod ctxs)).
-        rewrite <- List.map_id with (l:=(mds ++ List.map CMod.to_smod ctxs)) at 1.
+      - instantiate (1:=(mds ++ List.map UMod.to_smod ctxs)).
+        rewrite <- List.map_id with (l:=(mds ++ List.map UMod.to_smod ctxs)) at 1.
         eapply Forall2_apply_Forall2.
         { instantiate (1:=eq). admit "ez - ditto". }
         i. subst. exists gstb. split; ss. r. rewrite <- gstb_eq. refl.
@@ -241,6 +405,20 @@ Section ADQ.
     etrans.
     {
   Qed.
+
+
+
+
+
+
+
+
+
+
+
+
+
+
 
 
 
